examples/CSL/Allocator/Layout.v
@@ -25,12 +25,6 @@ Definition tag_retire : nat := 1.
 Definition tag_reclaim : nat := 2.
 Definition tag_retry : nat := 3.
 
-Definition page_metadata (base : nat) : list nat :=
-  [remote_head base; local_head base; drain_head base;
-   mailbox base false; mailbox base true].
-Definition page_cells (base capacity : nat) : list nat :=
-  page_metadata base ++ cells (page_blocks base capacity).
-
 Lemma page_size_positive capacity : Nat.lt 0 (page_size capacity).
 Proof. unfold page_size; lia. Qed.
 
@@ -60,67 +54,6 @@ Lemma page_blocks_link_payload_disjoint base capacity a b :
   a <> S b.
 Proof. apply node_addrs_link_payload_disjoint. Qed.
 
-Lemma page_metadata_range base x :
-  In x (page_metadata base) <-> Nat.le base x /\ Nat.lt x (base + 5).
-Proof.
-  unfold page_metadata, remote_head, local_head, drain_head, mailbox.
-  cbn [In]; lia.
-Qed.
-
-Lemma page_metadata_nodup base : NoDup (page_metadata base).
-Proof.
-  unfold page_metadata, remote_head, local_head, drain_head, mailbox.
-  repeat constructor; cbn [In]; intuition lia.
-Qed.
-
-
-Lemma mailbox_injective base client client' :
-  mailbox base client = mailbox base client' -> client = client'.
-Proof. destruct client, client'; unfold mailbox; intros H; try reflexivity; lia. Qed.
-
-Lemma page_metadata_blocks_disjoint base capacity x b :
-  In x (page_metadata base) -> In b (page_blocks base capacity) ->
-  x <> b /\ x <> S b.
-Proof.
-  intros Hx Hb; apply page_metadata_range in Hx.
-  apply page_blocks_bounds in Hb; lia.
-Qed.
-
-Lemma page_block_cells_range base capacity x :
-  In x (cells (page_blocks base capacity)) <->
-    Nat.le (base + 5) x /\ Nat.lt x (base + page_size capacity).
-Proof.
-  unfold page_blocks; rewrite node_cells_range; unfold page_size; lia.
-Qed.
-
-Lemma page_cells_range base capacity x :
-  In x (page_cells base capacity) <->
-    Nat.le base x /\ Nat.lt x (base + page_size capacity).
-Proof.
-  unfold page_cells; rewrite in_app_iff, page_metadata_range, page_block_cells_range.
-  unfold page_size; lia.
-Qed.
-
-(** This is the addresswise coverage useful for splitting metadata, links,
-    and payloads in the ownership invariant. *)
-Lemma page_interval_coverage base capacity x :
-  (Nat.le base x /\ Nat.lt x (base + page_size capacity)) <->
-    In x (page_metadata base) \/
-    exists b, In b (page_blocks base capacity) /\ (x = b \/ x = S b).
-Proof.
-  rewrite <- page_cells_range; unfold page_cells.
-  rewrite in_app_iff, in_cells; reflexivity.
-Qed.
-
-Lemma page_cells_nodup base capacity : NoDup (page_cells base capacity).
-Proof.
-  unfold page_cells; apply NoDup_app.
-  - apply page_metadata_nodup.
-  - apply node_addrs_cells_nodup.
-  - intros x Hmeta Hblock.
-    apply page_metadata_range in Hmeta.
-    apply page_block_cells_range in Hblock; lia.
-Qed.
 
 
 (** ** Pure counterparts of the checked initialization writes
@@ -194,19 +127,6 @@ Proof.
   - intro H; now left.
 Qed.
 
-Lemma page_heap_closed_none base capacity x :
-  page_heap base capacity hemp x = None <->
-    Nat.lt x base \/ Nat.le (base + page_size capacity) x.
-Proof.
-  split.
-  - intro Hnone; destruct (Nat.lt_ge_cases x base) as [Hlo | Hlo].
-    + now left.
-    + destruct (Nat.lt_ge_cases x (base + page_size capacity)) as [Hhi | Hhi].
-      * exfalso; apply (page_heap_in base capacity hemp x (conj Hlo Hhi)); exact Hnone.
-      * now right.
-  - intro Hout; rewrite page_heap_frame by exact Hout; reflexivity.
-Qed.
-
 
 Lemma page_heap_old_frame base capacity h :
   block_free h base (page_size capacity) ->
@@ -220,43 +140,6 @@ Proof.
     + apply page_heap_frame; now right.
 Qed.
 
-Lemma page_heap_on_page base capacity h f x :
-  (Nat.le base x /\ Nat.lt x (base + page_size capacity)) ->
-  page_heap base capacity h x = page_heap base capacity f x.
-Proof.
-  intro Hin; unfold page_heap; apply init_links_heap_lookup_agree.
-  repeat apply upd_lookup_agree.
-  rewrite (page_backing_in base capacity h x Hin).
-  rewrite (page_backing_in base capacity f x Hin); reflexivity.
-Qed.
-
-
-Lemma page_heap_split base capacity h :
-  heq (page_heap base capacity h) (hunion (page_heap base capacity hemp) h).
-Proof.
-  intro x; destruct (Nat.lt_ge_cases x base) as [Hlo | Hlo].
-  - rewrite hunion_none.
-    + apply page_heap_frame; now left.
-    + rewrite page_heap_frame by (now left); reflexivity.
-  - destruct (Nat.lt_ge_cases x (base + page_size capacity)) as [Hhi | Hhi].
-    + rewrite hunion_eq by (apply page_heap_in; split; assumption).
-      apply page_heap_on_page; split; assumption.
-    + rewrite hunion_none.
-      * apply page_heap_frame; now right.
-      * rewrite page_heap_frame by (now right); reflexivity.
-Qed.
-
-Lemma page_heap_disjoint base capacity h :
-  block_free h base (page_size capacity) ->
-  hdisj (page_heap base capacity hemp) h.
-Proof.
-  intros Hfree x; destruct (page_heap base capacity hemp x) eqn:E.
-  - right.
-    assert (Hin : Nat.le base x /\ Nat.lt x (base + page_size capacity)).
-    { apply page_heap_closed_dom; rewrite E; discriminate. }
-    replace x with (base + (x - base)) by lia; apply Hfree; lia.
-  - now left.
-Qed.
 
 Lemma page_heap_finite base capacity h :
   heap_finite h -> heap_finite (page_heap base capacity h).
@@ -304,23 +187,7 @@ Lemma page_heap_local_blocks base capacity h :
   page_heap base capacity h (local_head base) = Some (hd 0 (page_blocks base capacity)).
 Proof. rewrite page_heap_local; destruct capacity; reflexivity. Qed.
 
-Lemma page_heap_payload base capacity h b :
-  In b (page_blocks base capacity) -> page_heap base capacity h (S b) = Some 0.
-Proof.
-  intro Hb; pose proof (page_blocks_bounds base capacity b Hb) as Hbounds.
-  unfold page_heap; rewrite init_links_heap_payload by exact Hb.
-  unfold remote_head, local_head, drain_head, mailbox.
-  repeat rewrite upd_neq by lia.
-  apply page_backing_in; lia.
-Qed.
-
 Lemma page_heap_link base capacity h prefix b rest :
   page_blocks base capacity = prefix ++ b :: rest ->
   page_heap base capacity h b = Some (hd 0 rest).
 Proof. intro H; unfold page_heap; apply init_links_heap_link with (prefix := prefix); exact H. Qed.
-
-Lemma page_heap_link_index base capacity h j :
-  Nat.lt j capacity ->
-  page_heap base capacity h (base + 5 + 2 * j) =
-    Some (if Nat.ltb (S j) capacity then base + 5 + 2 * S j else 0).
-Proof. intro H; unfold page_heap; apply init_links_heap_link_index, H. Qed.
