theories/ICTree/Interp/State/Mod.v
@@ -148,58 +148,6 @@ Lemma interp_state_tau `{Encode E} `{Encode F} `(h: E ~> stateT W (ictree F)) {X
   interp_state h (Guard t) w ≅ Guard ((interp_state h t w)).
 Proof. rewrite !unfold_interp_state; reflexivity. Qed.
 
-(** [interp_state] applied on subevents, interprets the events leaving behind a subevent *)
-Definition h_resum `{Encode E1}`{Encode E2}`{Encode F}`{ReSum E1 E2}`{ReSumRet E1 E2} {W}
-  (h: E2 ~> stateT W (ictree F)): E1 ~> stateT W (ictree F) :=
-  fun (e: E1) =>
-    mkStateT
-      (fun w => runStateT (h (resum e)) w >>= fun '(x, w) => Ret (resum_ret e x, w)).
-
-Lemma interp_state_resumICtree`{Encode E1}`{Encode E2}`{Encode F}
-  `{ReSum E1 E2}`{ReSumRet E1 E2} {X} `(h: E2 ~> stateT W (ictree F)):
-  forall (t : ictree E1 X) (w : W),
-    interp_state h (resumICtree t) w ≅ interp_state (h_resum h) t w.
-Proof.
-  coinduction RR CIH; intros.
-  rewrite unfold_resumICtree, unfold_interp_state.
-  setoid_rewrite unfold_interp_state.
-  cbn.
-  desobs t; cbn.
-  - reflexivity.
-  - constructor.
-    intro i.
-    step.
-    constructor.
-    apply CIH.
-  - constructor.
-    apply CIH.
-  - cbn.
-    rewrite bind_bind.
-    upto_bind_equ.
-    destruct x.
-    rewrite bind_ret_l.
-    constructor.
-    apply CIH.
-Qed.
-
-(** Inversion lemma for [interp_state] applied on return values. *)
-Lemma interp_state_ret_inv `{Encode E} `{Encode F}
-  `(h: E ~> stateT W (ictree F)) {X}: forall s (t : ictree E X) r,
-    interp_state h t s ≅ Ret r -> t ≅ Ret (fst r) /\ s = snd r.
-Proof.
-  intros.
-  setoid_rewrite (ictree_eta t) in H1.
-  setoid_rewrite (ictree_eta t).
-  destruct (observe t) eqn:?.
-  - rewrite interp_state_ret in H1. step in H1. inv H1. split; reflexivity.
-  - rewrite interp_state_br in H1. step in H1. inv H1.
-  - rewrite interp_state_tau in H1. step in H1. inv H1.
-  - rewrite interp_state_vis in H1. apply ret_equ_bind in H1 as (? & ? & ?).
-    destruct x.
-    step in H2.
-    inv H2.
-Qed.
-
 (** [interp_state] applied on bind, commutes with the bind structure. *)
 Arguments interp_state: simpl never.
 Local Typeclasses Transparent equ.
@@ -231,18 +179,6 @@ Proof.
     rewrite bind_guard.
     constructor.
     apply IH.
-Qed.
-
-(** [interp_state] applied on map, commutes with the map structure. *)
-Lemma interp_state_map `{Encode E} `{Encode F} `(h : E ~> stateT W (ictree F))
-  {A B} (t : ictree E A) (f : A -> B) (s : W) :
-  interp_state h (ICtree.map f t) s ≅ ICtree.map (fun '(x, s) => (f x, s)) (interp_state h t s).
-Proof.
-  unfold ICtree.map.
-  rewrite interp_state_bind.
-  upto_bind_equ.
-  destruct x1.
-  apply interp_state_ret.
 Qed.
 
 (** [interp_state] applied on iteration, unfolds the iteration structure and commutes the interpretation inside the loop body. *)
@@ -294,23 +230,6 @@ Proof with eauto.
   reflexivity.
 Qed.
 
-(** [instr_stateE] is a special version of [interp_state] for the instrumentation monad.
-    Commutes with the bind structure. *)
-Lemma instr_state_bind {S A B} (t : ictree (stateE S) A) (k : A -> ictree (stateE S) B) (s : S) :
-  instr_stateE (t >>= k) s ≅ instr_stateE t s >>= fun '(x, s) => instr_stateE (k x) s.
-Proof.
-  unfold instr_stateE.
-  apply interp_state_bind.
-Qed.
-
-(** [instr_stateE] applied on map, commutes with the map structure. *)
-Lemma instr_state_map {S A B} (t : ictree (stateE S) A) (f : A -> B) (s : S) :
-  instr_stateE (ICtree.map f t) s ≅ ICtree.map (fun '(x, s) => (f x, s)) (instr_stateE t s).
-Proof.
-  unfold instr_stateE.
-  apply interp_state_map.
-Qed.
-
 (** [instr_state] applied on iteration, unfolds the iteration structure and interprets the loop body. *)
 Lemma instr_state_unfold_iter{S I R}
   (k : I -> ictree (stateE S) (I + R)) (i: I) (s: S) :
@@ -322,22 +241,6 @@ Lemma instr_state_unfold_iter{S I R}
 Proof.
   unfold instr_stateE.
   apply interp_state_unfold_iter.
-Qed.
-
-(** [instr_state] applied on get, returns the state. *)
-Lemma instr_state_get {S}: forall (s: S),
-  instr_stateE get s ~ Ret (s, s).
-Proof.
-  unfold instr_stateE.
-  apply interp_state_get.
-Qed.
-
-(** [instr_state] applied on put, interprets the event and the state leaving behind a log event. *)
-Lemma instr_state_put {S}: forall (s s': S),
-  instr_stateE (put s') s ~ log s' ;; Ret (tt, s').
-Proof with eauto.
-  unfold instr_stateE.
-  apply interp_state_put.
 Qed.
 
 (** * Interpreting one indexed emission.
